Logic/Modal/Standard/PLoN/Semantics.lean
@@ -41,78 +41,78 @@ end PLoN
 
 open Standard.PLoN
 
-def Formula.PLoN_Satisfies (M : PLoN.Model α) (w : M.World) : Formula α → Prop
+def Formula.plon_satisfies (M : PLoN.Model α) (w : M.World) : Formula α → Prop
   | atom a  => M.Valuation w a
   | verum   => True
   | falsum  => False
-  | and p q => (p.PLoN_Satisfies M w) ∧ (q.PLoN_Satisfies M w)
-  | or p q  => (p.PLoN_Satisfies M w) ∨ (q.PLoN_Satisfies M w)
-  | imp p q => (p.PLoN_Satisfies M w) → (q.PLoN_Satisfies M w)
-  | box p   => ∀ w', w ≺[p] w' → (p.PLoN_Satisfies M w')
+  | and p q => (p.plon_satisfies M w) ∧ (q.plon_satisfies M w)
+  | or p q  => (p.plon_satisfies M w) ∨ (q.plon_satisfies M w)
+  | imp p q => (p.plon_satisfies M w) → (q.plon_satisfies M w)
+  | box p   => ∀ w', w ≺[p] w' → (p.plon_satisfies M w')
 
 
-namespace Formula.PLoN_Satisfies
+namespace Formula.plon_satisfies
 
-protected instance instSemantics (M : PLoN.Model α) : Semantics (Formula α) (M.World) := ⟨fun w ↦ Formula.PLoN_Satisfies M w⟩
+protected instance instSemantics (M : PLoN.Model α) : Semantics (Formula α) (M.World) := ⟨fun w ↦ Formula.plon_satisfies M w⟩
 
 variable {M : PLoN.Model α} {w : M.World} {p q : Formula α}
 
-@[simp] protected lemma iff_models : w ⊧ p ↔ p.PLoN_Satisfies M w := by rfl
+@[simp] protected lemma iff_models : w ⊧ p ↔ p.plon_satisfies M w := by rfl
 
 instance : Semantics.Tarski M.World where
-  realize_top := by simp [PLoN_Satisfies];
-  realize_bot := by simp [PLoN_Satisfies];
-  realize_not := by simp [PLoN_Satisfies];
-  realize_and := by simp [PLoN_Satisfies];
-  realize_or  := by simp [PLoN_Satisfies];
-  realize_imp := by simp [PLoN_Satisfies];
+  realize_top := by simp [plon_satisfies];
+  realize_bot := by simp [plon_satisfies];
+  realize_not := by simp [plon_satisfies];
+  realize_and := by simp [plon_satisfies];
+  realize_or  := by simp [plon_satisfies];
+  realize_imp := by simp [plon_satisfies];
 
-end Formula.PLoN_Satisfies
+end Formula.plon_satisfies
 
 
-def Formula.PLoN_ValidOnModel (M : PLoN.Model α) (p : Formula α) : Prop := ∀ w : M.World, w ⊧ p
+def Formula.valid_on_PLoNModel (M : PLoN.Model α) (p : Formula α) : Prop := ∀ w : M.World, w ⊧ p
 
-namespace Formula.PLoN_ValidOnModel
+namespace Formula.valid_on_PLoNModel
 
-instance : Semantics (Formula α) (PLoN.Model α) := ⟨fun M ↦ Formula.PLoN_ValidOnModel M⟩
+instance : Semantics (Formula α) (PLoN.Model α) := ⟨fun M ↦ Formula.valid_on_PLoNModel M⟩
 
 @[simp]
-protected lemma Formula.PLoN_ValidOnModel.iff_models {M : PLoN.Model α} {p : Formula α}
-: M ⊧ p ↔ Formula.PLoN_ValidOnModel M p := by rfl
+protected lemma Formula.valid_on_PLoNModel.iff_models {M : PLoN.Model α} {p : Formula α}
+: M ⊧ p ↔ Formula.valid_on_PLoNModel M p := by rfl
 
 instance : Semantics.Bot (PLoN.Model α) where
-  realize_bot _ := by simp [Formula.PLoN_ValidOnModel];
+  realize_bot _ := by simp [Formula.valid_on_PLoNModel];
 
-end Formula.PLoN_ValidOnModel
+end Formula.valid_on_PLoNModel
 
 
-def Formula.PLoN_ValidOnFrame (F : PLoN.Frame α) (p : Formula α) := ∀ V, (Model.mk F V) ⊧ p
+def Formula.valid_on_PLoNFrame (F : PLoN.Frame α) (p : Formula α) := ∀ V, (Model.mk F V) ⊧ p
 
-namespace Formula.PLoN_ValidOnFrame
+namespace Formula.valid_on_PLoNFrame
 
-instance : Semantics (Formula α) (PLoN.Frame α) := ⟨fun F ↦ Formula.PLoN_ValidOnFrame F⟩
+instance : Semantics (Formula α) (PLoN.Frame α) := ⟨fun F ↦ Formula.valid_on_PLoNFrame F⟩
 
 @[simp]
-protected lemma Formula.PLoN_ValidOnFrame.iff_models {F : PLoN.Frame α} {p : Formula α}
-: F ⊧ p ↔ Formula.PLoN_ValidOnFrame F p := by rfl
+protected lemma Formula.valid_on_PLoNFrame.iff_models {F : PLoN.Frame α} {p : Formula α}
+: F ⊧ p ↔ Formula.valid_on_PLoNFrame F p := by rfl
 
 instance : Semantics.Bot (PLoN.Frame α) where
-  realize_bot _ := by simp [Formula.PLoN_ValidOnFrame];
+  realize_bot _ := by simp [Formula.valid_on_PLoNFrame];
 
-end Formula.PLoN_ValidOnFrame
+end Formula.valid_on_PLoNFrame
 
 
-def Formula.PLoN_ValidOnFrameClass (𝔽 : PLoN.FrameClass α) (p : Formula α) := ∀ (F : PLoN.Frame α), F ∈ 𝔽 → F ⊧ p
+def Formula.valid_on_PLoNFrameClass (𝔽 : PLoN.FrameClass α) (p : Formula α) := ∀ (F : PLoN.Frame α), F ∈ 𝔽 → F ⊧ p
 
-namespace Formula.PLoN_ValidOnFrameClass
+namespace Formula.valid_on_PLoNFrameClass
 
-instance : Semantics (Formula α) (PLoN.FrameClass α) := ⟨fun 𝔽 ↦ Formula.PLoN_ValidOnFrameClass 𝔽⟩
+instance : Semantics (Formula α) (PLoN.FrameClass α) := ⟨fun 𝔽 ↦ Formula.valid_on_PLoNFrameClass 𝔽⟩
 
 @[simp]
-protected lemma Formula.PLoN_ValidOnFrameClass.iff_models {𝔽 : PLoN.FrameClass α} {p : Formula α}
-: 𝔽 ⊧ p ↔ Formula.PLoN_ValidOnFrameClass 𝔽 p := by rfl
+protected lemma Formula.valid_on_PLoNFrameClass.iff_models {𝔽 : PLoN.FrameClass α} {p : Formula α}
+: 𝔽 ⊧ p ↔ Formula.valid_on_PLoNFrameClass 𝔽 p := by rfl
 
-end Formula.PLoN_ValidOnFrameClass
+end Formula.valid_on_PLoNFrameClass
 
 
 namespace PLoN
@@ -132,7 +132,7 @@ open Formula
 
 instance Definability.N : Definability (α := α) 𝐍 (λ _ => True) where
   defines := by
-    simp [System.theory, PLoN_ValidOnFrame, PLoN_ValidOnModel];
+    simp [System.theory, valid_on_PLoNFrame, valid_on_PLoNModel];
     intro F p hp;
     induction hp using Deduction.inducition_with_nec! with
     | hMaxm h => simp at h;
@@ -143,12 +143,12 @@ instance Definability.N : Definability (α := α) 𝐍 (λ _ => True) where
       intro V w w' _;
       exact ihp V w';
     | hDisj₃ =>
-      simp_all only [PLoN_Satisfies];
+      simp_all only [plon_satisfies];
       intros; rename_i hpr hqr hpq;
       cases hpq with
       | inl hp => exact hpr hp;
       | inr hq => exact hqr hq;
-    | _ => simp_all [PLoN_Satisfies];
+    | _ => simp_all [plon_satisfies];
 
 lemma FrameClassNonempty.N : Set.Nonempty (ℕ𝔽(𝐍) : PLoN.FrameClass α) := by
   existsi {World := PUnit, Rel := λ _ _ _ => True};
